examples/low-level/crypto/Crypto.AEAD.Wrappers.CMA.fst
@@ -24,56 +24,149 @@ module SeqProperties = FStar.SeqProperties
 module MAC = Crypto.Symmetric.MAC
 module EncodingWrapper = Crypto.AEAD.Wrappers.Encoding
 module PRF_MAC = Crypto.AEAD.PRF_MAC
+module RR = FStar.Monotonic.RRef
 
 (*** UF1CMA.mac ***)
 #reset-options "--z3rlimit 40 --initial_fuel 0 --max_fuel 0 --initial_ifuel 0 --max_ifuel 0"
-let mac_ensures (i:CMA.id) (st:CMA.state i) (acc:CMA.accBuffer i) (tag:MAC.tagB)
-		(h0:mem) (h1:mem) = 
-    let open FStar.Buffer in
-    let open Crypto.Symmetric.Bytes in
-    let open Crypto.Symmetric.Poly1305 in
-    let open Crypto.Symmetric.UF1CMA in
-    Buffer.live h0 st.s /\ 
-    MAC.live h0 st.r /\ 
-    Buffer.live h1 tag /\
-    CMA.acc_inv st acc h0 /\ (
-    if mac_log then
-      HS.modifies (Set.as_set [st.region; Buffer.frameOf tag]) h0 h1 /\
-      Buffer.modifies_buf_1 (Buffer.frameOf tag) tag h0 h1 /\
-      HS.modifies_ref st.region !{HS.as_ref (as_hsref (ilog st.log))} h0 h1 /\
-      m_contains (ilog st.log) h1 /\ (
-      let log = FStar.HyperStack.sel h1 (alog acc) in
-      let a = MAC.sel_elem h1 (abuf acc) in
-      let r = MAC.sel_elem h1 st.r in
-      let s = Buffer.as_seq h1 st.s in
-      let t = MAC.mac log r s in
-      sel_word h1 tag === t /\
-      snd (m_sel h1 (ilog st.log)) == Some(log,t))
-    else Buffer.modifies_1 tag h0 h1)
 
-let mac_wrapper (#i:CMA.id) (st:CMA.state i) (acc:CMA.accBuffer i) (tag:MAC.tagB)
+let mac_requires (#i:CMA.id) (ak:CMA.state i) (acc:CMA.accBuffer i) (tag:MAC.tagB) (h:mem) =
+  let open CMA in
+  let open HS in
+  EncodingWrapper.ak_acc_tag_separate ak acc tag /\
+  verify_liveness ak tag h /\
+  acc_inv ak acc h /\
+  (mac_log ==> Buffer.frameOf tag <> (alog acc).id) /\
+  (authId i ==> RR.m_sel h (ilog ak.log) == (snd i, None))
+
+(* let mac_ensures (i:CMA.id) (st:CMA.state i) (acc:CMA.accBuffer i) (tag:MAC.tagB) *)
+(* 		(h0:mem) (h1:mem) =  *)
+(*     let open FStar.Buffer in *)
+(*     let open Crypto.Symmetric.Bytes in *)
+(*     let open Crypto.Symmetric.Poly1305 in *)
+(*     let open Crypto.Symmetric.UF1CMA in *)
+(*     verify_liveness ak tag h1 /\ *)
+(*     acc_inv st acc h0 /\ ( *)
+(*     if mac_log then *)
+(*       HS.modifies (Set.as_set [st.region; Buffer.frameOf tag]) h0 h1 /\ *)
+(*       Buffer.modifies_buf_1 (Buffer.frameOf tag) tag h0 h1 /\ *)
+(*       HS.modifies_ref st.region !{HS.as_ref (as_hsref (ilog st.log))} h0 h1 /\ *)
+(*       m_contains (ilog st.log) h1 /\ ( *)
+(*       let log = FStar.HyperStack.sel h1 (alog acc) in *)
+(*       let a = MAC.sel_elem h1 (abuf acc) in *)
+(*       let r = MAC.sel_elem h1 st.r in *)
+(*       let s = Buffer.as_seq h1 st.s in *)
+(*       let t = MAC.mac log r s in *)
+(*       sel_word h1 tag === t /\ *)
+(*       snd (m_sel h1 (ilog st.log)) == Some(log,t)) *)
+(*     else Buffer.modifies_2 tag h0 h1) *)
+
+
+let modifies_bufs_and_ref (#a:Type) (#b:Type) (#c:Type)
+    (buf1:Buffer.buffer a)
+    (buf2:Buffer.buffer b{Buffer.frameOf buf1 = Buffer.frameOf buf2})   //this is true from CMA.state
+    (reff:HS.reference c{HH.disjoint HS.(reff.id) (Buffer.frameOf buf1)})  //this is stronger than you have currently ...
+    		   		 		 	  // ... but is true in the caller's context
+    h0 h1 : GTot Type0 =
+ let open FStar.HyperStack in
+ let open FStar.Buffer in
+ HS.modifies (Set.as_set [frameOf buf1; reff.id]) h0 h1 /\
+ HS.modifies_ref reff.id !{HS.as_ref reff} h0 h1 /\
+ HS.modifies_ref (frameOf buf1) !{HS.as_ref (Buffer.content buf1),
+				  HS.as_ref (Buffer.content buf2)} h0 h1
+
+let mac_modifies 
+        (i:id) (iv:Cipher.iv (Cipher.algi i))
+	(tbuf:lbuffer (v MAC.taglen))
+	(ak:CMA.state (i, iv))
+	(acc:CMA.accBuffer (i, iv)) 
+	(h0 h1:mem) = 
+  let abuf = MAC.as_buffer (CMA.abuf acc) in
+  if safeMac i 
+  then let log = RR.as_hsref CMA.(ilog ak.log) in
+       Buffer.frameOf abuf = Buffer.frameOf tbuf /\
+       HH.disjoint (Buffer.frameOf abuf) HS.(log.id) /\
+       modifies_bufs_and_ref abuf tbuf log h0 h1
+  else Buffer.modifies_2 abuf tbuf h0 h1
+
+let mac_wrapper (#i:EncodingWrapper.mac_id) (ak:CMA.state i) (acc:CMA.accBuffer i) (tag:MAC.tagB)
   : ST unit
-  (requires (fun h0 ->
-    let open Crypto.Symmetric.UF1CMA in
-    Buffer.live h0 tag /\ 
-    Buffer.live h0 st.s /\
-    Buffer.disjoint_2 (MAC.as_buffer (abuf acc)) st.s tag /\
-    Buffer.disjoint (MAC.as_buffer st.r) tag /\
-    Buffer.disjoint st.s tag /\ 
-    acc_inv st acc h0 /\
-    (mac_log ==> m_contains (ilog st.log) h0) /\
-    (mac_log /\ authId i ==> snd (m_sel h0 (ilog st.log)) == None)))
-  (ensures (fun h0 _ h1 -> mac_ensures i st acc tag h0 h1))
-  = let open Crypto.Symmetric.UF1CMA in
-    assume false; //TODO: this is out of date
-    let h0 = get () in
-    CMA.mac #i st acc tag;
-    let h1 = get () in 
-    if mac_log then begin
-      (* Need to update UF1CMA to prove this (problem with the mods clause not working fully) *)
-      assume (HS.modifies_ref st.region !{HS.as_ref (as_hsref (ilog st.log))} h0 h1) //NS: this goes away when UF1CMA is done
-    end
+  (requires (fun h0 -> mac_requires ak acc tag h0))
+  (ensures (fun h0 _ h1 -> CMA.mac_ensures i ak acc tag h0 h1 /\
+		        mac_modifies (fst i) (snd i) tag ak acc h0 h1))
+  = let h0 = get () in
+    CMA.mac #i ak acc tag; 
+    admit()
 
+(* let mac_ensures  *)
+(*         (i:id)  *)
+(*         (iv:Cipher.iv (Cipher.algi i)) *)
+(* 	(st:aead_state i Writer) *)
+(* 	(#aadlen:aadlen) (aad:lbuffer (v aadlen)) *)
+(* 	(#txtlen:txtlen_32) (plain:plainBuffer i (v txtlen)) *)
+(* 	(cipher_tagged:lbuffer (v txtlen + v MAC.taglen)) *)
+(* 	(ak:CMA.state (i, iv))  *)
+(* 	(acc:CMA.accBuffer (i, iv)) *)
+(* 	(h0 h1:mem) =  *)
+(*   enc_dec_liveness st aad plain cipher_tagged h1 /\ *)
+(*   mac_modifies i iv cipher_tagged ak acc h0 h1 /\  *)
+(*   (safeMac i ==> *)
+(*      h1 `HS.contains` (PRF.itable i st.prf) /\ ( *)
+(*      let prf_table = HS.sel h1 (PRF.itable i st.prf) in *)
+(*      let ad = Buffer.as_seq h1 aad in *)
+(*      let cbuf = Buffer.sub cipher_tagged 0ul txtlen in *)
+(*      let tbuf = Buffer.sub cipher_tagged txtlen MAC.taglen in *)
+(*      let cipher : lbytes (v txtlen) = Buffer.as_seq h1 cbuf in  *)
+(*      let tag : MAC.tag = Buffer.as_seq h1 tbuf in *)
+(*      mac_is_set prf_table iv ad (v txtlen) cipher tag h1)) *)
+     
+(* val mac (#i:EncodingWrapper.mac_id)  *)
+(* 	(st:aead_state (fst i) Writer) *)
+(* 	(#aadlen:aadlen) (aad:lbuffer (v aadlen)) *)
+(* 	(#txtlen:txtlen_32) (plain:plainBuffer (fst i) (v txtlen)) *)
+(* 	(cipher_tagged:lbuffer (v txtlen + v MAC.taglen)) *)
+(* 	(ak:CMA.state i)  *)
+(* 	(acc:CMA.accBuffer i) *)
+(* 	(h_init:mem) *)
+(*    : ST unit *)
+(*    (requires (fun h0 ->  *)
+(*      let open CMA in *)
+(*      let cipher : lbuffer (v txtlen) = Buffer.sub cipher_tagged 0ul txtlen in *)
+(*      let tag = Buffer.sub cipher_tagged txtlen MAC.taglen in *)
+(*      HS.is_stack_region HS.(h0.tip) /\ *)
+(*      enc_dec_separation st aad plain cipher_tagged /\ *)
+(*      enc_dec_liveness st aad plain cipher_tagged h0 /\ *)
+(*      EncodingWrapper.ak_acc_tag_separate ak acc tag /\ *)
+(*      EncodingWrapper.accumulate_ensures ak aad cipher h_init acc h0 /\ *)
+(*      verify_liveness ak tag h0 /\ *)
+(*      acc_inv ak acc h0 /\ *)
+(*      (authId i ==> RR.m_sel h0 (ilog ak.log) == (snd i, None)))) *)
+(*    (ensures (fun h0 _ h1 ->  *)
+(*       mac_ensures (fst i) (snd i) st aad plain cipher_tagged ak acc h0 h1)) *)
+(* #reset-options "--z3rlimit 100 --initial_fuel 0 --max_fuel 0 --initial_ifuel 0 --max_ifuel 0" *)
+(* open FStar.HyperStack *)
+(* open FStar.Buffer *)
+				  
+ 
+ 
+(*  		 	  		    (TSet.singleton (Buff buf2))) h0 h1 *)
+
+(* let mac #i st #aadlen aad #txtlen plain cipher_tagged ak acc h_init =       *)
+(*    let tag = Buffer.sub cipher_tagged txtlen MAC.taglen in *)
+(*    let h0 = get () in *)
+(*    mac_wrapper ak acc tag; *)
+(*    let h1 = get () in *)
+(*    assert (mac_modifies (fst i) (snd i) cipher_tagged ak acc h0 h1); *)
+(*    let abuf = MAC.as_buffer (CMA.abuf acc) in *)
+(*    FStar.Classical.move_requires (FStar.Buffer.lemma_reveal_modifies_2 abuf tag h0) h1; *)
+(*    assert (enc_dec_liveness st aad plain cipher_tagged h1); *)
+(*    admit() *)
+   
+
+(*    admit() *)
+
+    
+     
+	
 (*** UF1CMA.verify ***)
 
 (*+ The main work of wrapping UF1CMA.verify is to 
