examples/low-level/crypto/Crypto.AEAD.Wrappers.Encoding.fst
@@ -78,7 +78,53 @@ unfold let accumulate_ensures' (#i: MAC.id) (st: CMA.state i)
 let ak_acc_tag_separate (#i:CMA.id) (ak:CMA.state i) (acc:CMA.accBuffer i) (tag:lbuffer 16) =
     let open Crypto.Symmetric.UF1CMA in
     Buffer.disjoint_2 (MAC.as_buffer (abuf acc)) ak.s tag /\
-    Buffer.disjoint_2 (MAC.as_buffer ak.r) ak.s tag
+    Buffer.disjoint_2 (MAC.as_buffer ak.r) ak.s tag /\
+    Buffer.disjoint ak.s tag
+
+let ak_aad_cipher_separate (#i:CMA.id) (ak:CMA.state i) 
+		    (#aadlen:aadlen_32) (aad:lbuffer (v aadlen))
+		    (#n:nat) (cipher:lbuffer n) =
+    let open Crypto.Symmetric.UF1CMA in
+    Buffer.disjoint_2 (MAC.as_buffer ak.r) aad cipher
+
+let is_iv n (i:id) = UInt128.v n < pow2 (v (8ul *^ Cipher.ivlen (Cipher.algi i)))
+let mac_id = i:MAC.id{is_iv (snd i) (fst i)}
+let is_ak_for_iv (#i: mac_id) (#rw:rw) (aead_st:aead_state (fst i) rw) (ak:CMA.state i) (h:mem) =
+    let j = fst i in
+    let n = snd i in
+    safeId j ==> is_mac_for_iv #j #rw #n aead_st ak h
+    
+val accumulate_enc 
+	       (#i: mac_id) (#rw:rw) (aead_st:aead_state (fst i) rw)
+	       (ak: CMA.state i) (#aadlen:aadlen_32) (aad:lbuffer (v aadlen))
+	       (#txtlen:txtlen_32) (plain:plainBuffer (fst i) (v txtlen)) 
+	       (cipher_tagged:lbuffer (v txtlen + v MAC.taglen))
+   : StackInline (CMA.accBuffer i)
+      (requires (fun h0 -> 
+	  enc_dec_separation aead_st aad plain cipher_tagged /\
+	  enc_dec_liveness aead_st aad plain cipher_tagged h0 /\ 
+	  ak_aad_cipher_separate ak aad cipher_tagged /\
+	  PRF_MAC.ak_live PRF.(aead_st.prf.mac_rgn) ak h0))(*  /\ *)
+	  (* is_ak_for_iv aead_st ak h0)) *)
+      (ensures (fun h0 acc h1 ->  
+	  let tag : lbuffer (v MAC.taglen) = Buffer.sub cipher_tagged txtlen MAC.taglen in
+	  let cipher : lbuffer (v txtlen) = Buffer.sub cipher_tagged 0ul txtlen in
+      	  ak_acc_tag_separate ak acc tag /\
+	  enc_dec_liveness aead_st aad plain cipher_tagged h1 /\ 
+	  PRF_MAC.ak_live PRF.(aead_st.prf.mac_rgn) ak h1 /\
+	  (* is_ak_for_iv aead_st ak h1 /\	   *)
+	  accumulate_modifies_nothing h0 h1 /\
+	  accumulate_ensures ak aad cipher h0 acc h1))
+#reset-options "--z3rlimit 400 --initial_fuel 0 --max_fuel 0 --initial_ifuel 0 --max_ifuel 0"
+let accumulate_enc #i #rw aead_st ak #aadlen aad #txtlen plain cipher_tagged =	  
+    let h0 = get () in
+    let cipher : lbuffer (v txtlen) = Buffer.sub cipher_tagged 0ul txtlen in
+    let acc = accumulate ak aadlen aad txtlen cipher in
+    let h1 = get () in
+    assume (mac_log ==> fresh_sref h0 h1 (CMA.alog acc));
+    assume (fresh_sref h0 h1 (Buffer.content (MAC.as_buffer (CMA.abuf acc))));
+    FStar.Buffer.lemma_reveal_modifies_0 h0 h1;
+    acc
 
 let accumulate (#i: id) (#rw:rw) (#n:Cipher.iv (Cipher.algi i)) (aead_st:aead_state i rw)
 	       (ak: CMA.state (i, n)) (#aadlen:aadlen_32) (aad:lbuffer (v aadlen))
