examples/low-level/crypto/Crypto.AEAD.Encrypt.fst
@@ -1,0 +1,106 @@
+module Crypto.AEAD.Encrypt
+open FStar.UInt32
+open FStar.Ghost
+open Buffer.Utils
+open FStar.Monotonic.RRef
+
+open Crypto.Indexing
+open Crypto.Symmetric.Bytes
+open Crypto.Plain
+open Flag
+
+open Crypto.Symmetric.PRF
+open Crypto.AEAD.Encoding 
+open Crypto.AEAD.Invariant
+
+module HH       = FStar.HyperHeap
+module HS       = FStar.HyperStack
+module MAC      = Crypto.Symmetric.MAC
+module CMA      = Crypto.Symmetric.UF1CMA
+module Plain    = Crypto.Plain
+module Cipher   = Crypto.Symmetric.Cipher
+module PRF      = Crypto.Symmetric.PRF
+module Enxor    = Crypto.AEAD.EnxorDexor
+module PRF_MAC     = Crypto.AEAD.PRF_MAC
+module Encoding    = Crypto.AEAD.Encoding   
+module EncodingWrapper = Crypto.AEAD.Wrappers.Encoding
+module CMAWrapper = Crypto.AEAD.Wrappers.CMA
+
+////////////////////////////////////////////////////////////////////////////////
+#reset-options "--z3rlimit 400 --initial_fuel 0 --max_fuel 0 --initial_ifuel 0 --max_ifuel 0"
+let encrypt_ensures  (#i:id) (st:aead_state i Writer)
+		     (n: Cipher.iv (alg i))
+		     (#aadlen:aadlen)
+		     (aad: lbuffer (v aadlen))
+		     (#plainlen: UInt32.t)
+		     (plain: plainBuffer i (v plainlen))
+		     (cipher_tagged:lbuffer (v plainlen + v MAC.taglen))
+		     (h0:mem) (h1:mem) = 
+    enc_dec_liveness st aad plain cipher_tagged h1 /\
+    (safeMac i ==>  (
+       let aad = Buffer.as_seq h1 aad in
+       let p = Plain.sel_plain h1 plainlen plain in
+       let c = Buffer.as_seq h1 cipher_tagged in
+       HS.sel h1 st.log == SeqProperties.snoc (HS.sel h0 st.log) (AEADEntry n aad (v plainlen) p c)))
+       
+val encrypt:
+          i: id -> 
+ 	 st: aead_state i Writer ->
+          n: Cipher.iv (alg i) ->
+     aadlen: aadlen_32 ->
+        aad: lbuffer (v aadlen) ->
+   plainlen: txtlen_32 {safelen i (v plainlen) (otp_offset i)} ->
+      plain: plainBuffer i (v plainlen) ->
+ cipher_tag: lbuffer (v plainlen + v MAC.taglen) ->
+        ST  unit
+ (requires (fun h ->
+	enc_dec_separation st aad plain cipher_tag /\
+	enc_dec_liveness st aad plain cipher_tag h /\
+	fresh_nonce_st n st h /\
+	inv st h))
+  (ensures (fun h0 _ h1 ->
+	enc_dec_liveness st aad plain cipher_tag h1 /\
+	inv st h1 /\
+	encrypt_ensures st n aad plain cipher_tag h0 h1 /\
+	HS.modifies_transitively (Set.as_set [st.log_region; Buffer.frameOf cipher_tag]) h0 h1))
+	
+let encrypt i st n aadlen aad plainlen plain cipher_tagged =
+  assume (plainlen <> 0ul); //TODO: remove this; currently cannot encrypt empty plain texts
+  let h_init = get() in
+  push_frame(); 
+  let h0 = get () in
+  frame_inv_push st h_init h0; //inv st h0
+
+  let cipher : lbuffer (v plainlen) = Buffer.sub cipher_tagged 0ul plainlen in
+  let tag = Buffer.sub cipher_tagged plainlen MAC.taglen in
+  let x_0 = PRF.({iv = n; ctr = ctr_0 i}) in // PRF index to the first block
+
+  //call prf_mac: get a mac key, ak
+  let ak = PRF_MAC.prf_mac_enc st aad plain cipher_tagged st.ak x_0 in  // used for keying the one-time MAC
+  let h1 = get () in
+
+  //call enxor: fragment the plaintext, call the prf, and fill in the cipher text
+  Enxor.enxor n st aad plain cipher_tagged;
+  let h2 = get () in
+
+  assume (PRF_MAC.ak_live st.prf.mac_rgn ak h2); //provable, but slow
+
+  //call accumulate: encode the ciphertext and additional data for mac'ing 
+  let acc = EncodingWrapper.accumulate_enc #(i, n) st ak aad plain cipher_tagged in
+  
+  let h3 = get () in
+  admit()
+  
+  Buffer.lemma_reveal_modifies_0 h2 h3;
+  //call mac: filling in the tag component of the out buffer
+  mac_wrapper #(i,n) ak acc tag;
+  admit()
+
+(* (\* start: ideal and proof steps, to finish up, notably writing to the AEAD table  *\) *)
+(*   finish_after_mac h0 h3 i st n aadlen aad plainlen plain cipher_tagged ak acc tag; *)
+(* (\* end *\) *)
+
+(*   let h5 = get () in   *)
+(*   pop_frame(); //clean up any local allocation on our stack *)
+(*   encrypt_ensures_push_pop i st n aadlen aad plainlen plain cipher_tagged h_init h0 h5 *)
+
